<section xml:id="sec_abstractcft2">
  <title>The abstract reciprocity map </title>
  <introduction>
    <p>
      We next define the reciprocity map in abstract class field theory (<xref ref="def-abstract-recip-final"/>).
      As a bonus, this definition will give an explicit recipe for computing the reciprocity map in 
      local class field theory, but we will not expand on this point.
    </p>
  </introduction>
  <subsection xml:id="subsec-abstract-recip-definition">
  <title>Construction of the reciprocity map</title>
    <p>
      In order to define a candidate <m>r: \Gal(L/K) \to A_K/\Norm_{L/K} A_L</m> for the reciprocity map,
      we must first give a partial definition using a different domain.
    </p>
    <definition xml:id="def-abstract-recip-candidate">
      <p>
        Under <xref ref="hypo-abstract-cft"/>, let <m>L/K</m> be a Galois extension of finite subextensions of <m>\kbar/k</m>.
        Let <m>H</m> be the semigroup of
        <m>g \in \Gal(L^{\unr}/K)</m> such that <m>d_K(g)</m> is a positive integer.
        Define the map 
        <me>r': H \to A_K/\Norm_{L/K} A_{L}</me> 
        as follows.
        For <m>g \in \Gal(L^{\unr}/K)</m>,
        let <m>M</m> be the fixed field of <m>g</m>,
        so that
        <me>
          e(M/K) = e((M \cap L)/K), \qquad f(M/K) = d_K(g).
        </me>
        We may set <m>r'(g) = \Norm_{M/K} (\pi_M)</m> for some uniformizer <m>\pi_M</m> for <m>M</m>,
        once we check that this doesn't depend on the choice of <m>\pi_M</m>.
        To wit, if <m>\pi'_M</m> is another uniformizer for <m>M</m>,
        then <m>\pi_M/\pi'_M \in U_L</m> belongs to <m>\Norm_{L^{\unr}/L} U_{L^{\unr}}</m> by <xref ref="C_abstract_unramified"/>,
        so <m>\Norm_{M/K} (\pi_M/\pi'_M)</m> belongs to <m>\Norm_{L^{\unr}/K} U_{L^{\unr}} \subseteq \Norm_{L/K} U_L</m>.
        So at least <m>r'</m> is now a well-defined map, if not yet a semigroup homomorphism.
      </p>
    </definition>
    <remark xml:id="rmk-abstract-recip-properties">
      <p>
        Before getting into the weeds,
        let's make some other observations about <xref ref="def-abstract-recip-candidate"/>.
      </p>
      <p>
        First, <m>r'</m> is invariant under conjugation:
        if we replace <m>g</m> by <m>h^{-1}gh</m>,
        then its fixed field <m>M</m> is replaced by <m>M^h</m> and we can take the uniformizer <m>\pi_M^h</m>.
      </p>
      <p>
        Next, if <m>g \in H</m> is actually in <m>\Gal(L^{\unr}/L)</m>,
        then <m>r'(g) \in \Norm_{L/K} A_L</m>.
        In that case, <m>M</m> contains <m>L</m>,
        so <m>r'(g) = \Norm_{M/K}(\pi_M)</m> can be rewritten as
        <m>\Norm_{L/K} \Norm_{M/L} (\pi_M) \in \Norm_{L/K} A_L</m>.
        That is, if <m>r'</m> were known to be multiplicative,
        it would induce a group homomorphism from
        <m>\Gal(L/K)</m> to <m>A_K/\Norm_{L/K} A_L</m>.
      </p>
    </remark>
    <p>
      The remaining difficulty is to check that <m>r'</m> is multiplicative. 
      The issue here is that the definition of <m>r'(g)</m> involves taking the norm from a field extension that
      depends on <m>g</m>, so it is hopeless to directly compare different values of <m>g</m>.
      Instead, we rewrite the definition in a more uniform manner.
    </p>
    <proposition xml:id="prop_norm">
      <statement>
        <p>
          With notation as in <xref ref="def-abstract-recip-candidate"/>, put <m>n = d_K(g)</m> and choose <m>\phi \in H</m> with <m>d_K(\phi) = 1</m>.
          Then for <m>x \in A_M</m>,
          <me>
            \Norm_{M/K}(x) = \Norm_{L^{\unr}/K^{\unr}}(x x^\phi \cdots x^{\phi^{n-1}}).
          </me>
        </p>
      </statement>
      <proof>
        <p>
          Put <m>U = M \cap K^{\unr}</m>, so that <m>\Norm_{M/K} = \Norm_{U/K} \circ \Norm_{M/U}</m>.
          The group <m>\Gal(U/K)</m> is of order <m>n</m> generated by <m>\phi</m>, so for <m>y \in A_U</m>
          we have <m>\Norm_{U/K}(y) = y y^\phi \cdots y^{\phi^{n-1}}.</m>
          Meanwhile, on <m>A_M</m> we can view <m>\Norm_{M/U}</m> as the restriction of <m>\Norm_{L^{\unr}/K^{\unr}}</m>,
          so <m>\Norm_{M/U}(x) = \Norm_{L^{\unr}/K^{\unr}}(x)</m>. By taking <m>y = \Norm_{M/U}(x)</m> and rewriting
          <m>y^{\phi^i}</m> as <m>\Norm_{L^{\unr}/K^{\unr}}(x)^{\phi^i} = \Norm_{L^{\unr}/K^{\unr}}(x^{\phi^i})</m>,
          we deduce the claim.
        </p>
      </proof>
    </proposition>
    <p>
      Using the formula from <xref ref="prop_norm"/>, we can now establish multiplicativity.
    </p>
    <lemma xml:id="lem-abstract-recip-multiplicative">
      <statement>
        <p>
          The map <m>r': H \to A_K/\Norm_{L/K} A_L</m> exhibited in <xref ref="def-abstract-recip-candidate"/> is a homomorphism of semigroups.
        </p>
      </statement>
      <proof>
        <p>
          Let <m>g_1, g_2 \in H</m> be arbitrary and put <m>g_3 = g_1g_2</m>.
          Let <m>M_i</m> be the fixed field of <m>g_i</m>,
          let <m>\pi_i</m> be a uniformizer of <m>M_i</m>,
          and put <m>\rho_i = r'(g_i) = \Norm_{M_i/K}(\pi_i)</m>.
          Our goal is to check that
          <me>
            \rho_1\rho_2/\rho_3 \in \Norm_{L/K} A_{L}.
          </me>
          To begin with, note that
          <me>
            v_K(\rho_i) = f(M_i/K) v_{M_i}(\pi_i) = f(M_i/K) = d_K(g_i),
          </me>
          which implies that <m>v_K(\rho_1 \rho_2 /\rho_3) = 0</m>.
        </p>
        <p>
          Choose <m>\phi \in H</m> such that <m>d_K(\phi) = 1</m>.
          Put <m>d_i = d_K(g_i)</m> and 
          <me>
            \sigma_i = \pi_i \pi_i^\phi \cdots \pi_i^{\phi^{d_i-1}} \in M_i;
          </me>
          by <xref ref="prop_norm"/>, we have <m>\rho_i = \Norm_{L^{\unr}/K^{\unr}}(\sigma_i)</m>.
        </p>
        <p>
          Put <m>u = \sigma_1 \sigma_2/\sigma_3</m>.
          Let <m>N</m> be a finite unramified extension of <m>L</m> such that <m>u \in U_N</m>,
          so that 
          <me>
            \rho_1 \rho_2/\rho_3 = \Norm_{L^{\unr}/K^{\unr}}(u) = \Norm_{N/N \cap K^{\unr}}(u).
          </me>
          Since this quantity belongs to <m>K</m>, we may apply <xref ref="lem-intermediate-norm"/> to deduce that
          <me>
            \Norm_{L^{\unr}/K^{\unr}}(u) \in \Norm_{N/K} U_N \subset \Norm_{L/K} A_L,
          </me>
          as desired.
        </p>
      </proof>
    </lemma>
    <definition xml:id="def-abstract-recip-final">
      <p>
        With notation as in <xref ref="def-abstract-recip-candidate"/>,
        by combining <xref ref="def-abstract-recip-candidate"/>, <xref ref="rmk-abstract-recip-properties"/>, and
        <xref ref="lem-abstract-recip-multiplicative"/>, we obtain a semigroup homomorphism
        <m>r': H \to A_K/\Norm_{L/K}A_L</m> which kills <m>\Gal(L^{\unr}/L)</m>
        and thus induces a homomorphism <m>r = r_{L/K}: \Gal(L/K) \to A_K/\Norm_{L/K}A_L</m>.
        We call <m>r_{L/K}</m> the <term>reciprocity map</term>.
      </p>
    </definition>
    <p>
      Here are some consequences of the construction whose proofs are left to the reader.
   </p>
    <proposition xml:id="P_abstract_functorialities">
      <statement>
        <p>
          Under <xref ref="hypo-abstract-cft"/>, 
          if <m>L/K</m> and <m>L'/K'</m> are Galois extensions of finite subextensions of <m>\kbar/k</m> such that
          <m>K \subseteq K'</m> and <m>L \subseteq L'</m>,
          then the diagram in <xref ref="fig-abstractcft-4"/> commutes.
        </p>
          <figure xml:id="fig-abstractcft-4">
          <image>
          <latex-image>
          \xymatrix{
          \Gal(L'/K')^{\ab} \ar^{r_{L'/K'}}[r] \ar[d] &amp; A_{K'}/\Norm_{L'/K'} A_{L'} \ar^{\Norm_{K'/K}}[d] \\
          \Gal(L/K)^{\ab} \ar^{r_{L/K}}[r] &amp; A_K/\Norm_{L/K} A_L
          }
          </latex-image>
          </image>
          </figure>
      </statement>
    </proposition>
    <proposition xml:id="P_abstract_functorialities2">
      <statement>
        <p>
          Under <xref ref="hypo-abstract-cft"/>, 
          if <m>L/K</m> is a Galois extension of finite subextensions of <m>\kbar/k</m> 
          and <m>K'</m> is an intermediate field, then the diagram in <xref ref="fig-abstractcft-5"/> commutes.
          Here <m>V: \Gal(L/K)^{\ab} \to \Gal(L/K')^{\ab}</m> denotes the transfer map for the inclusion
          <m>\Gal(L/K') \subseteq \Gal(L/K)</m> (<xref ref="T_transfer_homomorphism"/>).
        </p>
          <figure xml:id="fig-abstractcft-5">
          <image>
          <latex-image>
          \xymatrix{
          \Gal(L/K)^{\ab} \ar^{r_{L/K}}[r] \ar^{V}[d] &amp; A_{K}/\Norm_{L/K} A_{L} \ar[d] \\
          \Gal(L/K')^{\ab} \ar^{r_{L/K'}}[r] &amp; A_{K'}/\Norm_{L/K'} A_{L}
          }
          </latex-image>
          </image>
          </figure>
      </statement>
      <proof>
        <p>
          See <xref ref="exer-abstract-functorialities2"/>.
        </p>
      </proof>
    </proposition>
  </subsection>
  <exercises>
    <title>Exercises</title>
     <exercise xml:id="exer-abstract-functorialities">
        <statement>
          Prove <xref ref="P_abstract_functorialities"/>.
        </statement>
        <hint>
          <p>
          See <xref ref="bib-Neukirch"/>, Proposition IV.5.8.
          </p>
        </hint>
      </exercise>
     <exercise xml:id="exer-abstract-functorialities2">
        <statement>
          Prove <xref ref="P_abstract_functorialities2"/>.
        </statement>
        <hint>
          <p>
          See <xref ref="bib-Neukirch"/>, Proposition IV.5.9.
          </p>
        </hint>
      </exercise>
      <exercise xml:id="exer-rescale-reciprocity">
        <statement>
          Under <xref ref="hypo-abstract-cft"/>, choose <m>c \in \widehat{\ZZ}^*</m> and let <m>s_{L/K}</m> be the reciprocity map defined using <m>cd</m> instead of <m>d</m>.
          Show that <m>s_{L/K} = c^{-1} r_{L/K}</m>.
        </statement>
      </exercise>
      <exercise xml:id="exer-rescale-reciprocity2">
        <statement>
          Under <xref ref="hypo-abstract-cft"/>, choose <m>c \in \widehat{\ZZ}^*</m> which acts on <m>\im(v)</m>, and let <m>s_{L/K}</m> be the reciprocity map defined 
          using <m>cd, cv</m> instead of <m>d, v</m>. Show that <m>s_{L/K} = r_{L/K}</m>.
        </statement>
      </exercise>
  </exercises>
</section>
